refactoring, putting old material in folder

src/StateMonad.v
@@ -1,287 +1,104 @@
-(** * The state monad *)
-
+Add LoadPath "./" as Monads .
+Require Import Monads.FunctorApplicativeMonad.
 Require Import NPeano Arith Bool String List.
-Require Import Coq.Logic.FunctionalExtensionality.
-
-Set Implicit Arguments.
-
-Class Monad(M:Type -> Type) := 
-{
-  ret : forall {A:Type}, A -> M A ; 
-  bind : forall {A B:Type}, M A -> (A -> M B) -> M B
-}.
-
-Notation "x <- c1 ;; c2" := (bind c1 (fun x => c2)) 
-                             (right associativity, at level 84, c1 at next level).
-
-Notation "c1 ;; c2" := (bind c1 (fun _ => c2)) (at level 100, right associativity).
 
 Axiom functional_extensionality : forall {X Y: Type}
                                     {f g : X -> Y},
   (forall (x:X), f x = g x) -> f = g.
 
-(** We now use a more refined definition for [state]: it is no more just an integer accounting for the 
-total number of computations needed to evaluate a term, but a [map] from [string] to [nat]. *)
+Definition state_comp(s:Type)(A:Type) := s -> (A*s).
 
-(** [ 
-]
-From Wadler's paper, we read: 
-
-_There is an important difference between the way monads are used in 
-the previous section and the way monads are used here. 
-The previous section showed monads help to use existing language 
-features more effectively; this section shows how monads can help define new language features. 
-No change to the programming language is required, but the implementation must provide a 
-new abstract data type, perhaps as part of the standard prelude.
-Here monads are used to manipulate state internal to the program_. *)
-
-Definition state := string -> nat.
-
-Definition newarray (n : nat) : state :=
-  (fun _ => n).
-
-Notation "'_' '!->' v" := (newarray v)
-  (at level 100, right associativity).
-
-Definition eqb_string (x y : string) : bool :=
-  if string_dec x y then true else false.
-
-Definition state_update  (m : state )
-                    (x : string) (v : nat) :=
-  fun x' => if eqb_string x x' then v else m x'.
-
-Definition empty_st := (_ !-> 0).
-
-(** It will also be useful to consider the [type] [unit], which has the property of having only one 
-inhabitant. To mimic Wadler's notation, we shall denote such an inhabitant with [()]. *)
-
-Notation "()" := tt.
-
-(** As for the [StateMonad] seen earlier, we define the [state_comp] function, which, given a type [A], 
-constructs a new type [state_comp A], which is a map [state -> (A*state)]. *)
-
-Definition state_comp(A:Type) := state -> (A*state).
-
-(** The definition below is identical to the one we have already seen, but where [state] is not just a [nat]. 
-A such, the statements and the corresponding proofs of the monad properties can be copied verbatim. *)
-
-Instance StateMonad : Monad state_comp := {
-  ret := fun {A:Type} (x:A) => (fun (s:state) => (x, s)) ; 
-  bind := fun {A B:Type} (c : state_comp A) (f: A -> state_comp B) => 
-            fun (s:state) => 
-              let (v, s') := c s in 
-              f v s'
-}.
-
-Lemma m_left_id_state_monad : forall {A B:Type} (x:A) (f:A -> state_comp B), bind (ret x) f = f x .
-Proof. intros. simpl. apply functional_extensionality. trivial. Qed. 
-
-Lemma m_right_id_state_monad : forall {A B:Type} (c:state_comp A), bind c ret = c. 
-Proof. intros. simpl. apply functional_extensionality. intros. destruct c. trivial. Qed.  
-
-Lemma m_assoc_state_monad : forall {A B C} (c:state_comp A) (f:A->state_comp B) (g:B -> state_comp C), 
-    bind (bind c f) g = bind c (fun x => bind (f x) g).
-Proof. intros. simpl. apply functional_extensionality. intros. destruct (c x). trivial. Qed.
+Definition state_comp_map {s} {a b} (f : a -> b) (r : state_comp s a)
+  : (state_comp s b):=
+fun x => (f (fst (r x)),snd(r x)).
 
 
+Lemma state_functor_identity {a} {s} (r : state_comp s a)
+  : state_comp_map id r = id r.
+Proof. intros. unfold state_comp_map.  apply functional_extensionality. intros. 
+unfold id.  destruct (r x). auto. Qed.
 
-(** 
-You might argue that building all this for the simple term language we have used to far as running
-example is an overkill and might not even make sense. You are right: we something a bit more sophisticated. 
-For this purpose, we are going to use a simplified version of [IMP], the simple imperative language we have 
-been working on in the _Formal Methods_ course. We want to complicate things, but not too much: we therefore 
-limit ourselves to considering expression which are: 
-- natural numbers 
-- variable IDs
-- sum of expressions 
-- equations between expressions. *)
-
-Inductive exp : Type :=
-  | ANum (n : nat)
-  | AId (x : string)             
-  | APlus (a1 a2 : exp)
-  | EqExp (a1 a2: exp).
-
-Coercion AId : string >-> exp.
-Coercion ANum : nat >-> exp.
-
-Declare Custom Entry com.
-Declare Scope com_scope.
-Notation "<{ e }>" := e (at level 0, e custom com at level 99) : com_scope.
-Notation "( x )" := x (in custom com, x at level 99) : com_scope.
-Notation "x" := x (in custom com at level 0, x constr at level 0) : com_scope.
-Notation "f x .. y" := (.. (f x) .. y)
-                  (in custom com at level 0, only parsing,
-                  f constr at level 0, x constr at level 9,
-                  y constr at level 9) : com_scope.
-Notation "x + y" := (APlus x y) (in custom com at level 50, left associativity).
-Notation "x == y" := (EqExp x y) (in custom com at level 50, left associativity).
-Open Scope com_scope.
-
-Definition X:string:="x"%string.
-Definition Y:string:="y"%string.
-Definition Z:string:="z"%string.
-
-(** As far as commands go, we consider: 
-- the "skip" command, which performs no action
-- the assignment command, which assigns an expression to a variable
-- the sequence of two commands
-- the [If] statement.
-
-*)
-
-Inductive com : Type :=
-  | CSkip 
-  | CAss (x : string) (a : exp)
-  | CSeq (c1 c2 : com)
-  | CIf (a: exp) (c1 c2 : com).
-
-Notation "'skip'"  :=
-         CSkip (in custom com at level 0) : com_scope.
-Notation "x := y"  :=
-         (CAss x y)
-            (in custom com at level 0, x constr at level 0,
-             y at level 85, no associativity) : com_scope.
-Notation "x ; y" :=
-         (CSeq x y)
-           (in custom com at level 90, right associativity) : com_scope.
-Notation "'if' x 'then' y 'else' z 'end'" :=
-         (CIf x y z)
-           (in custom com at level 89, x at level 99,
-            y at level 99, z at level 99) : com_scope.
-
-(** We now need two functions that allow us to interact with states: 
-- the function [block]: the call [block n m] creates a new state with all locations initialised to [n],
- applies monad [m] to this initial state to yield value [a] and final state [x], deallocates the array, and returns [a].
-- the function [fetch]: the call [fetch x] returns the value at index [x] (indices in our case are just strings)
- in the current state, and leaves the state unchanged.
-- the function [assign]: the call [assign x n] returns the empty value [()],
- and updates the state so that index [x] contains value [n].*)
-
-Definition block{A:Type} (n:nat) (m: state_comp A): A :=
-let (a,_):= m (newarray n) in a.
-
-Definition fetch (x:string) : state_comp nat := 
-  fun s => (s x, s).
-
-Definition assign (x:string) (n:nat) : state_comp unit := 
-  fun s => ((), state_update s x n).
-
-(** In contrast with the previous section, in the code below, we first present implementations of [eval] and 
-[exec] that do not make use of the concept of monad, as they might the easier to read, especially if one
-keeps in mind the how we have defined small/big step semantics for IMP. *)
-
-Fixpoint eval_no_monad (a : exp)(s: state): nat :=
-  match a with
-  | ANum n       => n
-  | AId x        => s x                                
-  | <{a1 + a2}>  => (eval_no_monad a1 s) + (eval_no_monad a2 s)
-  | <{a1 == a2}> => let n1 := eval_no_monad a1 s in 
-                            let n2:= eval_no_monad a2 s in if (beq_nat n1 n2) then 0 else 1 end.
-
-Fixpoint exec_no_monad (c : com)(s: state) : state :=
-  match c with
-  | <{ skip }>                    => s
-  | <{ x := a }>                  => let n:= eval_no_monad a s in state_update s x n
-  | <{c1; c2}>                    => exec_no_monad c2 (exec_no_monad c1 s)
-  | <{if a then c1 else c2 end}>  => let n:= eval_no_monad a s in
-                                                      match n with 
-                                                        | 0 => exec_no_monad c1 s
-                                                        | _ => exec_no_monad c2 s
-                                                      end
-  end.
-
-Compute eval_no_monad <{Z + 1}> empty_st.
-
-Definition fact_in_coq : com :=
-  <{ Z := X;
-     Y := 1;
-     if Z == 0 then
-       Y := Y + Z
-      else
-       Z := Z + 1
-     end
-     }>.
-
-Compute exec_no_monad fact_in_coq empty_st X.
-Compute exec_no_monad fact_in_coq empty_st Y.
-
-(** Let us now define [eval] and [exec] using the State Monad. We first evaluate expressions: evaluation of a term 
-returns a [nat] and may access or modify the state.
-In fact, evaluation only accesses the state and never alters it. The intepretation, e.g. in the case of 
-addition, goes as follows: [eval (<{a1 + a2}>)] tells you to compute the evaluation of [a1],
-bind [n1] to the result, then compute the evaluation of [a2], bind [n1] to the result, then return [n1 + n2]. 
-*)
-
-Fixpoint eval (a : exp) : state_comp nat :=
-  match a with
-  | ANum n       => ret n
-  | AId x        => fetch x                                
-  | <{a1 + a2}>  => n1 <- eval a1 ;; n2 <- eval a2 ;; ret (n1 + n2)
-  | <{a1 == a2}> => n1 <- eval a1 ;; n2 <- eval a2 ;; if (beq_nat n1 n2) then ret 0 else ret 1 end.
+Lemma state_functor_composition_identity {a b c} {s}
+  (u : b -> c) (v : a -> b) (r : state_comp s a)
+  : state_comp_map  (u <<< v) r = ((state_comp_map  u) <<< (state_comp_map  v)) r.
+Proof. unfold state_comp_map. apply functional_extensionality. intros. unfold compose.
+destruct (r x). auto. Qed.
 
 
-(** We now define execution on commands: note that, as opposed to [eval],
-execution of a command returns nothing and may access or modify the state. How do we interpret the code 
-below? In the case of a sequence of commands, we have that [exec <{c1; c2}>] tells you to 
-compute the execution of [c1], then compute the execution of [c2], then return nothing. *)
+#[program]
+Instance state_Functor (s : Type) 
+  : Functor (state_comp s ) :=
+  { map := @state_comp_map s  
+  }.
+  
+Next Obligation. apply state_functor_identity. Defined.
 
-Fixpoint exec (c : com) : state_comp unit :=
-  match c with
-  | <{ skip }>                    => ret ()
-  | <{ x := a }>                  => n <- eval a ;; assign x n 
-  | <{c1; c2}>                    => x <- exec c1 ;; y <- exec c2 ;; ret ()
-  | <{if a then c1 else c2 end}>  => n <- eval a ;;
-                                    match n with 
-                                      | 0 => exec c1
-                                      | _ => exec c2 
-                                    end
-  end.
+Definition state_comp_apply {s}{a b} (f : state_comp s (a -> b)) (fs : state_comp s a)
+  : state_comp s b := 
+  fun s => let (x, s'):= fs s in let (g, s''):= f s' in (g x, s'').
+
+Definition state_comp_pure {s} {a}(x:a) : state_comp s a :=
+fun s => (x, s).
+
+Lemma state_comp_applicative_identity {s} {a}
+  (v : state_comp s  a):
+  state_comp_apply (state_comp_pure id) v = v.
+  Proof. unfold state_comp_apply. apply functional_extensionality. intros. 
+destruct (v x). unfold state_comp_pure. auto. Qed.
+
+Lemma state_comp_applicative_homomorphism {s} {a b} (v : a -> b) (x : a)
+  : state_comp_apply (state_comp_pure v) (state_comp_pure x) = state_comp_pure (s:=s) (v x).
+Proof. unfold state_comp_apply. apply functional_extensionality. intros. 
+unfold state_comp_pure. auto. Qed.
+
+Lemma state_comp_applicative_interchange {s}{a b}(u : state_comp s (a -> b)) (y : a)
+  : state_comp_apply u (state_comp_pure y) = state_comp_apply (state_comp_pure (fun z : a -> b => z y)) u.
+
+Proof. unfold state_comp_apply. apply functional_extensionality. intros. 
+unfold state_comp_pure. auto. Qed.
+
+#[program]
+Instance state_Applicative {s}
+  : Applicative (state_comp s) :=
+  { pure := @state_comp_pure s 
+  ; apply := @state_comp_apply s 
+  }.
+  
+Next Obligation. apply state_comp_applicative_identity. Defined.
+Next Obligation. unfold state_comp_apply, state_comp_pure.
+apply functional_extensionality. intros.  destruct (w x). destruct (v s0). 
+destruct (u s1). auto. Defined.
+Next Obligation. unfold state_comp_apply, state_comp_pure, state_comp_map.
+apply functional_extensionality. intros. destruct (x x0). auto. Defined.
+
+Definition state_comp_bind {s} {a b}
+  (r : state_comp s a) (f : a -> state_comp s b)
+  : state_comp s b :=
+  fun s => 
+              let (v, s') := r s in 
+              f v s'.
+
+Lemma state_bind_associativity {s} {a b c} 
+  (f : state_comp s a) (g : a -> state_comp s b) (h : b -> state_comp s c)
+  : state_comp_bind (state_comp_bind f g) h = 
+  state_comp_bind f (fun x : a => state_comp_bind (g x) h).
+Proof. unfold state_comp_bind. apply functional_extensionality. intros. 
+destruct (f x). destruct (g a0). trivial. Qed.
+
+#[program]
+Instance state_comp_Monad {s}
+  : Monad (state_comp s) :=
+  { bind := @state_comp_bind s
+  }.
+  
+Next Obligation. unfold state_comp_bind, state_comp_pure. 
+apply functional_extensionality. intros.
+destruct (x x0). trivial. Defined.
+Next Obligation. apply state_bind_associativity. Defined.
+Next Obligation. unfold state_comp_bind, state_comp_map, state_comp_pure.
+apply functional_extensionality. intros. destruct (x x0). trivial. Defined.
 
 
-Compute snd (exec fact_in_coq empty_st) X.
-Compute snd (exec fact_in_coq empty_st) Y.
-
-(**  As a final step, we prove that [eval] is equivalent to [eval_no_monad] and that 
-[exec] is equivalent to [exec_no_monad]. *)
-
-Lemma eval_not_mod_state: forall a s, snd (eval a s) = s.
-Proof. intros. induction a; try auto; 
-simpl; destruct (eval a1 s); unfold snd in IHa1; rewrite IHa1; 
-destruct (eval a2 s); unfold snd in *; try destruct (n =? n0); assumption.
-Qed.
-
-Theorem eval_equiv: forall e s, eval_no_monad e s = fst (eval e s).
-Proof. intros. induction e; try auto.
-- simpl. rewrite IHe1. rewrite IHe2.  remember (eval e1 s). 
-apply (f_equal snd) in Heqp. rewrite eval_not_mod_state in Heqp. apply eq_sym in Heqp.
- destruct (eval e1 s).   rewrite Heqp. subst. destruct p. unfold snd. destruct (eval e2 s). auto.
-- simpl. rewrite IHe1. rewrite IHe2.  remember (eval e1 s). 
-apply (f_equal snd) in Heqp. rewrite eval_not_mod_state in Heqp. apply eq_sym in Heqp.
-destruct (eval e1 s).   rewrite Heqp. subst. destruct p. unfold snd. destruct (eval e2 s). 
-unfold fst.
-destruct (fst (n0, s) =? fst (n1, s1)); destruct (n0 =? n1); auto. Qed.
-
-Theorem exec_equiv: forall c s, exec_no_monad c s = snd (exec c s).
-Proof. intros. generalize dependent s. induction c; try auto.
-
-- intros. simpl. rewrite eval_equiv.  remember (eval a s). apply (f_equal snd) in Heqp.
-rewrite eval_not_mod_state in Heqp. destruct (eval a s). destruct p. unfold snd in Heqp.
-subst.  unfold fst. unfold assign. unfold snd. auto.
-
-- intros. simpl. rewrite IHc1.  rewrite IHc2. remember (exec c1 s).
-destruct p. unfold snd.  destruct (exec c2 s0). auto. 
-
-- intros. simpl.  rewrite eval_equiv. rewrite IHc1.  rewrite IHc2. 
-remember (eval a s). apply (f_equal snd) in Heqp. rewrite eval_not_mod_state in Heqp. 
-destruct p. unfold snd in Heqp. subst. unfold fst. destruct n; auto. Qed.
-
-
-(**  From Wadler we read: _How a functional language may provide in-place array update is an old problem. 
-This section has presented a new solution, consisting of two abstract data types with eight operations between them. 
-No change to the programming language is required, other than to provide an implementation of these types, 
-perhaps as part of the standard prelude. The discovery of such a simple solution comes as a surpise, 
-considering the plethora of more elaborate solutions that have been proposed_. *)
 
 
 
