src/StateMonadApplications.v
@@ -1,5 +1,5 @@
 Add LoadPath "./" as Monads .
-Require Import Monads.ParametricStateMonad.
+Require Import Monads.StateMonad.
 Require Import Monads.FunctorApplicativeMonad.
 Require Import NPeano Arith Bool String List.
 
